rename

ground_zero/cubical.lean
@@ -4,7 +4,7 @@ namespace ground_zero
 open ground_zero.HITs ground_zero.types
 open ground_zero.HITs.interval (i₀ i₁ seg)
 
-namespace path
+namespace Path
 
 universes u v r s
 
@@ -13,8 +13,8 @@ inductive binary (α : Sort u) : ℕ → Type u
 | node {n : ℕ} : binary n → binary n → binary (n + 1)
 
 def interval_cube : ℕ → Type
-| 0 := 𝕀
-| (n + 1) := interval_cube n × 𝕀
+| 0 := I
+| (n + 1) := interval_cube n × I
 
 def construct_cube {α : Sort u} :
   Π {n : ℕ}, (interval_cube n → α) → binary α n
@@ -23,39 +23,38 @@ def construct_cube {α : Sort u} :
   (construct_cube (λ n, f ⟨n, i₀⟩))
   (construct_cube (λ n, f ⟨n, i₁⟩))
 
-inductive cube {α : Sort u} (n : ℕ) : binary α n → Type u
-| lam (f : interval_cube n → α) : cube (construct_cube f)
+inductive Cube {α : Sort u} (n : ℕ) : binary α n → Type u
+| lam (f : interval_cube n → α) : Cube (construct_cube f)
 
-def path {α : Sort u} (a b : α) := cube 0 (binary.leaf a b)
-def path.lam {α : Sort u} (f : 𝕀 → α) :
-  path (f i₀) (f i₁) :=
-cube.lam f
+def Path {α : Sort u} (a b : α) := Cube 0 (binary.leaf a b)
+def Path.lam {α : Sort u} (f : I → α) : Path (f i₀) (f i₁) :=
+Cube.lam f
 
-abbreviation lineP (σ : 𝕀 → Sort u) := Π (i : 𝕀), σ i
-abbreviation line (α : Sort u) := 𝕀 → α
-def line.refl {α : Sort u} (a : α) : line α := λ _, a
+abbreviation LineP (σ : I → Sort u) := Π (i : I), σ i
+abbreviation Line (α : Sort u) := I → α
+def Line.refl {α : Sort u} (a : α) : Line α := λ _, a
 
-def square {α : Sort u} (a b c d : α) :=
-cube 1 (binary.node (binary.leaf a b) (binary.leaf c d))
-def square.lam {α : Sort u} (f : 𝕀 → 𝕀 → α) :
-  square (f i₀ i₀) (f i₁ i₀) (f i₀ i₁) (f i₁ i₁) :=
-cube.lam (λ (x : interval_cube 1), product.elim f x)
+def Square {α : Sort u} (a b c d : α) :=
+Cube 1 (binary.node (binary.leaf a b) (binary.leaf c d))
+def Square.lam {α : Sort u} (f : I → I → α) :
+  Square (f i₀ i₀) (f i₁ i₀) (f i₀ i₁) (f i₁ i₁) :=
+Cube.lam (λ (x : interval_cube 1), product.elim f x)
 
-def from_equality {α : Sort u} {a b : α} (p : a = b :> α) : path a b :=
-path.lam (interval.rec a b p)
+def from_equality {α : Sort u} {a b : α} (p : a = b :> α) : Path a b :=
+Path.lam (interval.rec a b p)
 
-def to_equality {α : Sort u} {a b : α} (p : path a b) : a = b :> α :=
-@cube.rec α 0 (begin intros B p, cases B with a b, exact a = b :> α end)
+def to_equality {α : Sort u} {a b : α} (p : Path a b) : a = b :> α :=
+@Cube.rec α 0 (begin intros B p, cases B with a b, exact a = b :> α end)
   (λ f, f # seg) (binary.leaf a b) p
 
-def compute {α : Sort u} {a b : α} (p : path a b) : 𝕀 → α :=
+def compute {α : Sort u} {a b : α} (p : Path a b) : I → α :=
 interval.rec a b (to_equality p)
 
-def coe (π : 𝕀 → Sort u) (x : π i₀) : Π i, π i :=
+def coe (π : I → Sort u) (x : π i₀) : Π i, π i :=
 interval.ind x (equiv.subst seg x) eq.rfl
 
 infix ` # `:40 := compute
-notation `<` binder `> ` r:(scoped P, path.lam P) := r
+notation `<` binder `> ` r:(scoped P, Path.lam P) := r
 
 /-
                      p
@@ -70,22 +69,17 @@ notation `<` binder `> ` r:(scoped P, path.lam P) := r
           a -----------------> a
                    <i> a
   vertices are written from left to right, from bottom to top:
-    square a a a b
+    Square a a a b
 -/
-infix ` ⇝ `:30 := path
+infix ` ⇝ `:30 := Path
 
-def square.and {α : Sort u} {a b : α}
-  (p : a ⇝ b) : square a a a b :=
-square.lam (λ i j, p # i ∧ j)
+def Square.and {α : Sort u} {a b : α}
+  (p : a ⇝ b) : Square a a a b :=
+Square.lam (λ i j, p # i ∧ j)
 
-def square.const {α : Sort u} (a : α) :
-  square a a a a :=
-square.lam (λ i j, a)
-
-def square.mk {α : Sort u} {a₀ a₁ b₀ b₁ : α}
-  (u : a₀ ⇝ a₁) (v : b₀ ⇝ b₁)
-  (r₀ : a₀ ⇝ b₀) (r₁ : a₁ ⇝ b₁) :
-  square a₀ a₁ b₀ b₁ := sorry
+def Square.const {α : Sort u} (a : α) :
+  Square a a a a :=
+Square.lam (λ i j, a)
 
 structure tetrad (α : Sort u) (β : Sort v) (γ : Sort r) (δ : Sort s) :=
 (one : α) (two : β) (three : γ) (four : δ)
@@ -98,8 +92,8 @@ structure tetrad (α : Sort u) (β : Sort v) (γ : Sort r) (δ : Sort s) :=
 --    V         V
 --    b₀ -----> b₁
 --         v
-def square.extract {α : Sort u} {a b c d : α}
-  (s : square a b c d) : tetrad (a ⇝ b) (b ⇝ c) (c ⇝ d) (a ⇝ d) :=
+def Square.extract {α : Sort u} {a b c d : α}
+  (s : Square a b c d) : tetrad (a ⇝ b) (b ⇝ c) (c ⇝ d) (a ⇝ d) :=
 begin
   cases s with f, split,
   exact <i> f ⟨i, i₀⟩, exact <i> f ⟨−i, i⟩,
@@ -148,8 +142,8 @@ def comp_test₁ {α : Type u} {a b : α} (p : a ⇝ b) : (p # i₁) ⇝ b := rf
 
 -- fail
 --def symm_test {α : Type u} {a b : α} (p : a ⇝ b) : (p⁻¹)⁻¹ ⇝ p := rfl
-def trans {α : Type u} {a b c : α} (p : a ⇝ b) (q : b ⇝ c) : a ⇝ c :=
-subst q p
+@[trans] def trans {α : Type u} {a b c : α}
+  (p : a ⇝ b) (q : b ⇝ c) : a ⇝ c := subst q p
 
 infix ⬝ := trans
 
@@ -158,24 +152,15 @@ def comp {α : Type u} {a b c d : α}
   (bottom : b ⇝ c) (left : b ⇝ a) (right : c ⇝ d) : a ⇝ d :=
 left⁻¹ ⬝ bottom ⬝ right
 
-lemma eta {α : Type u} {a b : α} (p : a ⇝ b) :
-  (<i> p # i) = p :> a ⇝ b := begin
-  cases p with f, unfold path.lam,
-  have q : (λ i, cube.lam f # i) = f :> _ := begin
-    apply interval.funext, intro x,
-    refine interval.ind _ _ _ x,
-    repeat { reflexivity },
-    admit
-  end,
-  admit
-end
-
-def interval_contr (i : 𝕀) : i₀ ⇝ i := coe (λ i, i₀ ⇝ i) rfl i
+def interval_contr (i : I) : i₀ ⇝ i := coe (λ i, i₀ ⇝ i) rfl i
 def seg_path : i₀ ⇝ i₁ := interval_contr i₁
 
 def conn_and {α : Sort u} {a b : α} (p : a ⇝ b) :
-  Π (i : 𝕀), a ⇝ p # i :=
+  LineP (λ i, a ⇝ p # i) :=
 λ i, <j> p # i ∧ j
+
+def PathP (σ : I → Type u) (a : σ i₀) (b : σ i₁) :=
+Path (subst seg_path a) b
 
 --def J {α : Type u} {a : α} {π : Π (b : α), a ⇝ b → Type u}
 --  (h : π a (refl a)) (b : α) (p : a ⇝ b) : π b (<i> p # i) :=
@@ -185,7 +170,7 @@ def conn_and {α : Sort u} {a b : α} (p : a ⇝ b) :
 --  (h : π a (refl a)) (b : α) (p : a ⇝ b) : π b (<i> p # i) :=
 --transport (<i> π (p # i) (<j> p # i ∧ j)) h
 
-end path
+end Path
 
 namespace cubicaltt
 
@@ -202,11 +187,11 @@ def add_succ (a : ℕ) : Π (b : ℕ), add (nat.succ a) b ⇝ nat.succ (add a b)
 | (b + 1) := <i> nat.succ (add_succ b # i)
 
 def add_zero_inv : Π (a : ℕ), a ⇝ add a nat.zero :=
-path.refl
+Path.refl
 
 def add_comm (a : ℕ) : Π (b : ℕ), add a b ⇝ add b a
 | 0 := <i> (add_zero a) # −i
-| (b + 1) := path.comp (<i> nat.succ (add_comm b # i))
+| (b + 1) := Path.comp (<i> nat.succ (add_comm b # i))
                        (<j> nat.succ (add a b))
                        (<j> add_succ b a # −j)
 
@@ -216,7 +201,7 @@ def add_assoc (a b : ℕ) : Π (c : ℕ), add a (add b c) ⇝ add (add a b) c
 
 def add_comm₃ {a b c : ℕ} : add a (add b c) ⇝ add c (add b a) :=
 let r : add a (add b c) ⇝ add a (add c b) := <i> add a (add_comm b c # i) in
-path.comp (add_comm a (add c b)) (<j> r # −j) (<j> add_assoc c b a # −j)
+Path.comp (add_comm a (add c b)) (<j> r # −j) (<j> add_assoc c b a # −j)
 
 example (n m : ℕ) (h : n ⇝ m) : nat.succ n ⇝ nat.succ m :=
 <i> nat.succ (h # i)
