ground_zero/HITs/interval.lean
@@ -4,37 +4,37 @@ open ground_zero.HITs.trunc ground_zero.structures
 namespace ground_zero
 namespace HITs
 
-def 𝕀 := ∥bool∥
-abbreviation interval := 𝕀
+def I := ∥bool∥
+abbreviation interval := I
 
 namespace interval
   universes u v
 
-  def i₀ : 𝕀 := trunc.elem ff
-  def i₁ : 𝕀 := trunc.elem tt
-  def seg : i₀ = i₁ :> 𝕀 := trunc.uniq i₀ i₁
+  def i₀ : I := trunc.elem ff
+  def i₁ : I := trunc.elem tt
+  def seg : i₀ = i₁ :> I := trunc.uniq i₀ i₁
 
   abbreviation zero := i₀
   abbreviation one := i₁
 
   @[inline, recursor 4]
   def rec {β : Sort u} (b₀ : β) (b₁ : β)
-    (s : b₀ = b₁ :> β) : 𝕀 → β :=
+    (s : b₀ = b₁ :> β) : I → β :=
   let f (b : bool) : singl b₀ :=
     bool.rec (singl.trivial_loop b₀) ⟨b₁, s⟩ b in
   singl.point ∘ trunc.rec f
 
   /- β i₀ and β i₁ are Prop’s,
      so s : b₀ = b₁ is trivial -/
-  def hrec {β : 𝕀 → Prop} (b₀ : β i₀) (b₁ : β i₁) :
-    Π (x : 𝕀), β x := begin
+  def hrec {β : I → Prop} (b₀ : β i₀) (b₁ : β i₁) :
+    Π (x : I), β x := begin
     intros, refine trunc.ind _ _ x, intros,
     { induction a, apply b₀, apply b₁ },
     { intros, trivial }
   end
 
-  def ind {π : 𝕀 → Sort u} (b₀ : π i₀) (b₁ : π i₁)
-    (s : b₀ =[seg] b₁) : Π (x : 𝕀), π x := begin
+  def ind {π : I → Sort u} (b₀ : π i₀) (b₁ : π i₁)
+    (s : b₀ =[seg] b₁) : Π (x : I), π x := begin
     intro x, refine quot.hrec_on x _ _,
     { intro b, cases b, exact b₀, exact b₁ },
     { intros, induction s,
@@ -46,7 +46,7 @@ namespace interval
   end
 
   def homotopy {α : Sort u} {β : Sort v} {f g : α → β}
-    (p : f ~ g) (x : α) : 𝕀 → β :=
+    (p : f ~ g) (x : α) : I → β :=
   rec (f x) (g x) (p x)
 
   def funext {α : Sort u} {β : Sort v} {f g : α → β}
@@ -62,21 +62,21 @@ namespace interval
     {f g : Π (x : α), β x} (p : f = g :> _) : f ~ g :=
   begin induction p, apply types.equiv.homotopy.id end
 
-  instance : prop 𝕀 := ⟨trunc.uniq⟩
+  instance : prop I := ⟨trunc.uniq⟩
   instance trunc_functions {α : Type u} : prop (∥α∥ → ∥α∥) :=
   ⟨begin intros, apply funext, intro x, apply trunc.uniq end⟩
 
-  def neg : 𝕀 → 𝕀 :=
+  def neg : I → I :=
   trunc.rec (trunc.elem ∘ bnot)
   prefix `−`:20 := neg
 
-  def bool_to_interval (f : bool → bool → bool) (a b : 𝕀) : 𝕀 :=
+  def bool_to_interval (f : bool → bool → bool) (a b : I) : I :=
   trunc.rec (λ a, trunc.rec (trunc.elem ∘ f a) b) a
 
-  def min (a b : 𝕀) : 𝕀 :=
+  def min (a b : I) : I :=
   trunc.rec (begin intro x, cases x, exact i₀, exact a end) b
 
-  def max : 𝕀 → 𝕀 → 𝕀 := bool_to_interval bor
+  def max : I → I → I := bool_to_interval bor
 
   notation r `∧`:70 s := min r s
   notation r `∨`:70 s := max r s
